caseStudy/ADT/Cost.dfy
@@ -1,0 +1,25 @@
+/******************************************************************************
+  Abstract Cost type
+******************************************************************************/
+
+module Cost {
+
+  trait {:termination false} Cost<Input> {
+    ghost var t:nat
+    ghost const x:Input 
+
+    ghost method Inc()
+      modifies this
+      ensures t == old(t)+1 
+    {
+      t := t + 1;
+    }      
+
+    ghost function Input(): Input reads this { x }
+
+    ghost function Count(): nat reads this { t }   
+
+    ghost function Size(): nat reads this
+  }
+
+}
